proofs/GoLeanProofs/Adequacy.lean
@@ -77,7 +77,7 @@ abort on an unrecovered panic*". -/
 theorem go_adequacy [GoCoreGpreS .hasLC GF] (c : Config) (σ : ExecState)
     (φ : Unit → Prop) (hσwf : HeapWf σ)
     (Hwp : ∀ [GoCoreGS .hasLC GF], GoCoreGS.prog GF = σ.functions →
-      GoCoreGS.methods GF = σ.methods →
+      GoCoreGS.methods GF = σ.methods → GoCoreGS.types GF = σ.types →
       ⊢@{IProp GF} (WP c {{ v, ⌜φ v⌝ }})) :
     adequate .NotStuck c σ (fun v _ => φ v) := by
   refine wp_adequacy (GF := GF) .NotStuck c σ φ ?_
@@ -92,11 +92,12 @@ theorem go_adequacy [GoCoreGpreS .hasLC GF] (c : Config) (σ : ExecState)
       (Std.PartialMap.map (fun g : GName => toAgree (LeibnizO.mk g))
         (∅ : GoHeapF GName)))
     HeapView.auth_one_valid with ⟨%γm, Hm⟩
-  letI _ : GoCoreGS .hasLC GF := ⟨⟨γh, γm⟩, σ.functions, σ.methods⟩
+  letI _ : GoCoreGS .hasLC GF := ⟨⟨γh, γm⟩, σ.functions, σ.methods, σ.types⟩
   imodintro
   iexists (fun σ' _ =>
     iprop(genHeapInterp (GF := GF) (H := GoHeapF) (heapToMap σ'.heap)
-      ∗ ⌜σ'.functions = σ.functions ∧ σ'.methods = σ.methods ∧ HeapWf σ'⌝))
+      ∗ ⌜σ'.functions = σ.functions ∧ σ'.methods = σ.methods
+          ∧ σ'.types = σ.types ∧ HeapWf σ'⌝))
   iexists (fun _ => iprop(True))
   isplitl [Hh Hm]
   · isplitl [Hh Hm]
@@ -109,8 +110,8 @@ theorem go_adequacy [GoCoreGpreS .hasLC GF] (c : Config) (σ : ExecState)
       unfold ghost_map_auth
       iframe Hh Hm
     · ipureintro
-      exact ⟨rfl, rfl, hσwf⟩
-  · exact Hwp rfl rfl
+      exact ⟨rfl, rfl, rfl, hσwf⟩
+  · exact Hwp rfl rfl rfl
 
 /-! ## Arc `exit-infra` (2b): the strong-adequacy operational readout
 
@@ -135,10 +136,10 @@ theorem go_heap_adequacy [GoCoreGpreS .hasLC GF] (c : Config) (σ : ExecState)
     (Ψ : ∀ [GoCoreGS .hasLC GF], Unit → IProp GF)
     (φ : Unit → ExecState → Prop) (hσwf : HeapWf σ)
     (Hwp : ∀ [GoCoreGS .hasLC GF], GoCoreGS.prog GF = σ.functions →
-      GoCoreGS.methods GF = σ.methods →
+      GoCoreGS.methods GF = σ.methods → GoCoreGS.types GF = σ.types →
       ⊢@{IProp GF} (WP c {{ v, Ψ v }}))
     (Hext : ∀ [GoCoreGS .hasLC GF], GoCoreGS.prog GF = σ.functions →
-      GoCoreGS.methods GF = σ.methods →
+      GoCoreGS.methods GF = σ.methods → GoCoreGS.types GF = σ.types →
       ∀ (σ2 : ExecState) (v : Unit),
         iprop(genHeapInterp (GF := GF) (H := GoHeapF) (heapToMap σ2.heap) ∗ Ψ v)
           ⊢ |==> ⌜φ v σ2⌝) :
@@ -159,11 +160,12 @@ theorem go_heap_adequacy [GoCoreGpreS .hasLC GF] (c : Config) (σ : ExecState)
       (Std.PartialMap.map (fun g : GName => toAgree (LeibnizO.mk g))
         (∅ : GoHeapF GName)))
     HeapView.auth_one_valid with ⟨%γm, Hm⟩
-  letI _ : GoCoreGS .hasLC GF := ⟨⟨γh, γm⟩, σ.functions, σ.methods⟩
+  letI _ : GoCoreGS .hasLC GF := ⟨⟨γh, γm⟩, σ.functions, σ.methods, σ.types⟩
   imodintro
   iexists (fun σ' _ _ _ =>
     iprop(genHeapInterp (GF := GF) (H := GoHeapF) (heapToMap σ'.heap)
-      ∗ ⌜σ'.functions = σ.functions ∧ σ'.methods = σ.methods ∧ HeapWf σ'⌝))
+      ∗ ⌜σ'.functions = σ.functions ∧ σ'.methods = σ.methods
+          ∧ σ'.types = σ.types ∧ HeapWf σ'⌝))
   iexists [(fun v => Ψ v)], (fun _ => iprop(True)), (fun _ _ _ _ => fupd_intro)
   dsimp only
   isplitl [Hh Hm]
@@ -177,10 +179,10 @@ theorem go_heap_adequacy [GoCoreGpreS .hasLC GF] (c : Config) (σ : ExecState)
       unfold ghost_map_auth
       iframe Hh Hm
     · ipureintro
-      exact ⟨rfl, rfl, hσwf⟩
+      exact ⟨rfl, rfl, rfl, hσwf⟩
   isplitl
   · iapply BigSepL2.bigSepL2_singleton
-    exact Hwp rfl rfl
+    exact Hwp rfl rfl rfl
   iintro %es' %t2' %Heq %Hlen %HNS Hst Hwptp _
   icases BigSepL2.bigSepL2_cons_inv_right $$ Hwptp with ⟨%e', %_, %Heq', Hpost, H⟩
   subst Heq' Heq
@@ -192,7 +194,7 @@ theorem go_heap_adequacy [GoCoreGpreS .hasLC GF] (c : Config) (σ : ExecState)
     ipureintro
     grind
   · dsimp only [Option.elim_some]
-    imod (Hext rfl rfl σ2 _) $$ [$Hgh $Hpost] with %Hφv
+    imod (Hext rfl rfl rfl σ2 _) $$ [$Hgh $Hpost] with %Hφv
     iapply fupd_mask_intro_discard Std.LawfulSet.empty_subset
     ipureintro
     grind
@@ -209,11 +211,11 @@ theorem go_heap_adequacy_own [GoCoreGpreS .hasLC GF] (c : Config)
     (Ψ : ∀ [GoCoreGS .hasLC GF], Unit → IProp GF)
     (φ : Unit → ExecState → Prop) (hσwf : HeapWf σ)
     (Hwp : ∀ [GoCoreGS .hasLC GF], GoCoreGS.prog GF = σ.functions →
-      GoCoreGS.methods GF = σ.methods →
+      GoCoreGS.methods GF = σ.methods → GoCoreGS.types GF = σ.types →
       iprop([∗map] l ↦ cell ∈ heapToMap σ.heap, l ↦ cell)
         ⊢@{IProp GF} (WP c {{ v, Ψ v }}))
     (Hext : ∀ [GoCoreGS .hasLC GF], GoCoreGS.prog GF = σ.functions →
-      GoCoreGS.methods GF = σ.methods →
+      GoCoreGS.methods GF = σ.methods → GoCoreGS.types GF = σ.types →
       ∀ (σ2 : ExecState) (v : Unit),
         iprop(genHeapInterp (GF := GF) (H := GoHeapF) (heapToMap σ2.heap) ∗ Ψ v)
           ⊢ |==> ⌜φ v σ2⌝) :
@@ -226,21 +228,22 @@ theorem go_heap_adequacy_own [GoCoreGpreS .hasLC GF] (c : Config)
   iintro %Hinv
   imod (genHeap_init_names (GF := GF) (heapToMap σ.heap))
     with ⟨%γh, %γm, Hσ, Hpts, Htok⟩
-  letI _ : GoCoreGS .hasLC GF := ⟨⟨γh, γm⟩, σ.functions, σ.methods⟩
+  letI _ : GoCoreGS .hasLC GF := ⟨⟨γh, γm⟩, σ.functions, σ.methods, σ.types⟩
   imodintro
   iexists (fun σ' _ _ _ =>
     iprop(genHeapInterp (GF := GF) (H := GoHeapF) (heapToMap σ'.heap)
-      ∗ ⌜σ'.functions = σ.functions ∧ σ'.methods = σ.methods ∧ HeapWf σ'⌝))
+      ∗ ⌜σ'.functions = σ.functions ∧ σ'.methods = σ.methods
+          ∧ σ'.types = σ.types ∧ HeapWf σ'⌝))
   iexists [(fun v => Ψ v)], (fun _ => iprop(True)), (fun _ _ _ _ => fupd_intro)
   dsimp only
   isplitl [Hσ]
   · isplitl [Hσ]
     · iexact Hσ
     · ipureintro
-      exact ⟨rfl, rfl, hσwf⟩
+      exact ⟨rfl, rfl, rfl, hσwf⟩
   isplitl [Hpts]
   · iapply BigSepL2.bigSepL2_singleton
-    iapply (Hwp rfl rfl) $$ Hpts
+    iapply (Hwp rfl rfl rfl) $$ Hpts
   iintro %es' %t2' %Heq %Hlen %HNS Hst Hwptp _
   icases BigSepL2.bigSepL2_cons_inv_right $$ Hwptp with ⟨%e', %_, %Heq', Hpost, H⟩
   subst Heq' Heq
@@ -252,7 +255,7 @@ theorem go_heap_adequacy_own [GoCoreGpreS .hasLC GF] (c : Config)
     ipureintro
     grind
   · dsimp only [Option.elim_some]
-    imod (Hext rfl rfl σ2 _) $$ [$Hgh $Hpost] with %Hφv
+    imod (Hext rfl rfl rfl σ2 _) $$ [$Hgh $Hpost] with %Hφv
     iapply fupd_mask_intro_discard Std.LawfulSet.empty_subset
     ipureintro
     grind
@@ -272,7 +275,7 @@ theorem go_heap_invariance [GoCoreGpreS .hasLC GF] (c : Config)
     (σ : ExecState) (t2 : List Config) (σ2 : ExecState) (φ : Prop)
     (hσwf : HeapWf σ)
     (Hwp : ∀ [GoCoreGS .hasLC GF], GoCoreGS.prog GF = σ.functions →
-      GoCoreGS.methods GF = σ.methods →
+      GoCoreGS.methods GF = σ.methods → GoCoreGS.types GF = σ.types →
       iprop([∗map] l ↦ cell ∈ heapToMap σ.heap, l ↦ cell)
         ⊢ |={⊤}=> iprop(
             (WP c {{ _v, iprop(True) }}) ∗
@@ -285,19 +288,20 @@ theorem go_heap_invariance [GoCoreGpreS .hasLC GF] (c : Config)
   iintro %Hinv %κs
   imod (genHeap_init_names (GF := GF) (heapToMap σ.heap))
     with ⟨%γh, %γm, Hσ, Hpts, Htok⟩
-  letI _ : GoCoreGS .hasLC GF := ⟨⟨γh, γm⟩, σ.functions, σ.methods⟩
-  imod (Hwp rfl rfl) $$ Hpts with ⟨Hwp', Hcont⟩
+  letI _ : GoCoreGS .hasLC GF := ⟨⟨γh, γm⟩, σ.functions, σ.methods, σ.types⟩
+  imod (Hwp rfl rfl rfl) $$ Hpts with ⟨Hwp', Hcont⟩
   imodintro
   iexists (fun σ' _ _ =>
     iprop(genHeapInterp (GF := GF) (H := GoHeapF) (heapToMap σ'.heap)
-      ∗ ⌜σ'.functions = σ.functions ∧ σ'.methods = σ.methods ∧ HeapWf σ'⌝))
+      ∗ ⌜σ'.functions = σ.functions ∧ σ'.methods = σ.methods
+          ∧ σ'.types = σ.types ∧ HeapWf σ'⌝))
   iexists (fun _ => iprop(True))
   dsimp only
   isplitl [Hσ]
   · isplitl [Hσ]
     · iexact Hσ
     · ipureintro
-      exact ⟨rfl, rfl, hσwf⟩
+      exact ⟨rfl, rfl, rfl, hσwf⟩
   isplitl [Hwp']
   · iexact Hwp'
   iintro ⟨Hgh, %Hpure⟩
@@ -325,7 +329,7 @@ semantics, full stop. -/
 theorem adequate_seqn_nil (σ : ExecState) (env : LocalEnv) (hwf : HeapWf σ) :
     adequate .NotStuck (Config.exec (.seqn #[]) env .stop) σ (fun _ _ => True) :=
   go_adequacy (GF := GoCoreS) _ _ _ hwf (by
-    intro _ _ _
+    intro _ _ _ _
     iapply wp_seqn
     simp only [seqCont]
     iapply fupd_intro
